proof a general form of execute_body

examples/sbf/verif.v
@@ -159,6 +159,261 @@ Proof.
   entailer.
 Qed.
 
+(* This is the general form of RegisterAction's apply method's spec that we support.
+  We expecct this is general enough for all practical application. We don't support
+  other kind of apply methods. *)
+Definition RegisterAction_apply_spec (p : path) (w : N) (f : Z -> Z) (retv : Z -> Sval) : func_spec :=
+  WITH,
+    PATH p
+    MOD None []
+    WITH old_value (H_old_value : 0 <= old_value < Z.pow 2 (Z.of_N w)),
+      PRE
+        (ARG [ValBaseBit (P4Arith.to_loptbool w old_value)]
+        (MEM []
+        (EXT [])))
+      POST
+        (ARG_RET [ValBaseBit (P4Arith.to_loptbool w (f old_value));
+                  retv old_value]
+           ValBaseNull
+        (MEM []
+        (EXT []))).
+
+(* TODO write down the write post condition.
+  the problem here is, we need to say Znth i c is ValBaseBit, right? *)
+
+Definition RegisterAction_execute_spec : func_spec :=
+  WITH p (* path *) index_w w (* width *) s (* size *) r (* reg *)
+      (H_r : PathMap.get p (ge_ext ge) = Some (Tofino.EnvRegAction r))
+      (H_ws : PathMap.get r (ge_ext ge) = Some (Tofino.EnvRegister (w, s)))
+      (H_s : 0 <= s <= Z.pow 2 (Z.of_N index_w))
+      apply_fd apply_f apply_retv
+      (H_apply_fd : PathMap.get (p ++ ["apply"]) (ge_ext ge) =
+          Some (Tofino.EnvAbsMet (exec_abstract_method am_ge p apply_fd)))
+      (H_apply_body : fundef_satisfies_spec am_ge apply_fd nil
+          (RegisterAction_apply_spec p w apply_f apply_retv)),
+    PATH p
+    MOD None [r]
+    WITH (c : list Val) (i : Z)
+      (H_c : Zlength c = s)
+      (H_i : 0 <= i < s)
+      old_v
+      (H_old_v : Znth i c = ValBaseBit old_v /\ Zlength old_v = Z.of_N w),
+      PRE
+        (ARG [eval_val_to_sval (ValBaseBit (P4Arith.to_lbool index_w i))]
+        (MEM []
+        (EXT [ExtPred.singleton r (Tofino.ObjRegister c)])))
+      POST
+        (ARG_RET [] (apply_retv (P4Arith.BitArith.lbool_to_val old_v 1 0))
+        (MEM []
+        (EXT [ExtPred.singleton r
+            (Tofino.ObjRegister (upd_Znth i c
+                (ValBaseBit (P4Arith.to_lbool w (apply_f (P4Arith.BitArith.lbool_to_val old_v 1 0))))))]))).
+
+Ltac intros_fs_bind :=
+  repeat lazymatch goal with
+  | |- fundef_satisfies_spec _ _ _ (fs_bind (fun x => _)) =>
+    let x := fresh x in intro x
+  | |- fundef_satisfies_spec _ _ _ ?x =>
+    unfold x
+  end.
+
+Ltac intros_fsh_bind :=
+  repeat lazymatch goal with
+  | |- fundef_satisfies_hoare _ _ _ _ (fsh_bind (fun x => _)) =>
+    let x := fresh x in intro x
+  | |- fundef_satisfies_hoare _ _ _ _ ?x =>
+    unfold x
+  end.
+
+Lemma RegisterAction_execute_body :
+  fundef_satisfies_spec ge execute_fundef nil RegisterAction_execute_spec.
+Proof.
+  intros_fs_bind.
+  split.
+  2 : {
+    unfold func_modifies. intros.
+    inv H.
+    inv H5. inv H.
+    eapply eq_trans in H0; only 2 : (symmetry; apply H_r).
+    symmetry in H0; inv H0.
+    eapply eq_trans in H3; only 2 : (symmetry; apply H_ws).
+    symmetry in H3; inv H3.
+    eapply eq_trans in H1; only 2 : (symmetry; apply H_apply_fd).
+    symmetry in H1; inv H1.
+    destruct (-1 <? index) eqn:?.
+    2 : {
+      simpl in H8. destruct H8; subst.
+      apply modifies_refl.
+    }
+    destruct (index <? s) eqn:?.
+    2 : {
+      simpl in H8. destruct H8; subst.
+      apply modifies_refl.
+    }
+    simpl in H8. destruct H8; subst.
+    eapply modifies_trans.
+    { eapply modifies_incl.
+      { assert (modifies None [] (m, es) (m, s')). {
+          split.
+          { constructor. }
+          { simpl.
+            inv H7.
+            eapply (proj2 H_apply_body) in H1.
+            apply H1.
+          }
+        }
+        eassumption.
+      }
+      all : solve_modifies.
+    }
+    eapply modifies_set_ext with (st := (m, s')).
+    simpl.
+    replace (in_scope r r) with true. 2 : {
+      clear; induction r.
+      - auto.
+      - simpl. rewrite eqb_refl; auto.
+    }
+    auto.
+  }
+  intros_fsh_bind.
+  unfold fundef_satisfies_hoare.
+  unfold hoare_func; intros.
+  inv H0. inv H6.
+  inv H0.
+  eapply eq_trans in H1; only 2 : (symmetry; apply H_r).
+  symmetry in H1; inv H1.
+  eapply eq_trans in H4; only 2 : (symmetry; apply H_ws).
+  symmetry in H4; inv H4.
+  eapply eq_trans in H2; only 2 : (symmetry; apply H_apply_fd).
+  symmetry in H2; inv H2.
+  destruct H as [? []].
+  destruct H1 as [? _].
+  simpl in H1.
+  rewrite H5 in H1. inv H1.
+  assert (index = i). {
+    clear -H_i H_s H H3 H6.
+    unfold arg_denote, arg_satisfies in H.
+    inv H. inv H5.
+    inv H3. clear H7.
+    assert (ValBaseBit indexb = (ValBaseBit (P4Arith.to_lbool index_w i))). {
+      eapply exec_val_eq.
+      eapply exec_val_sym with eq.
+      { clear; auto. }
+      assert (val_to_sval
+          (ValBaseBit (P4Arith.to_lbool index_w i))
+          (eval_val_to_sval (ValBaseBit (P4Arith.to_lbool index_w i)))). {
+        eapply exec_val_sym with strict_read_ndetbit.
+        2 : eapply sval_to_val_eval_val_to_sval.
+        { clear; sauto. }
+        { clear; sauto. }
+      }
+      eapply exec_val_trans with (f := read_detbit);
+        [ | eapply exec_val_trans; [ | eassumption | eassumption] | eassumption ].
+      { unfold rel_trans; clear; sauto. }
+      { unfold rel_trans; clear; sauto. }
+    }
+    inv H.
+    rewrite P4Arith.bit_from_to_bool in H6.
+    inv H6.
+    apply Z.mod_small.
+    unfold P4Arith.BitArith.upper_bound.
+    lia.
+  }
+  clear H H3 H6.
+  subst.
+  destruct (-1 <? i) eqn:Heqb; only 2 : lia. clear Heqb.
+  destruct (i <? Zlength c) eqn:Heqb; only 2 : lia. clear Heqb.
+  simpl in H7. destruct H9. subst.
+  clear H0.
+  assert (content' = c). {
+    clear -H_apply_body H H5 H8.
+    inv H8.
+    apply (H_apply_body) in H1.
+    destruct H1.
+    assert (PathMap.get r s' = PathMap.get r es). {
+      symmetry.
+      apply H3.
+      auto.
+    }
+    rewrite H4 in H.
+    change (@extern_object Info (@Expression Info) (@extern_sem Info (@Expression Info) target))
+      with (@Tofino.object Info (@Expression Info)) in H.
+    congruence.
+  }
+  clear H H5.
+  subst.
+  destruct H_old_v.
+  set (old_value := P4Arith.BitArith.lbool_to_val old_v 1 0).
+  assert (new_value = ValBaseBit (P4Arith.to_lbool w (apply_f old_value))
+      /\ sval_to_val read_ndetbit (apply_retv old_value) retv). {
+    clear -H_apply_body H H0 H8.
+    inv H8.
+    eapply (proj1 H_apply_body old_value) in H2.
+    3 : {
+      split.
+      2 : { split; constructor. }
+      inv H1. inv H8.
+      rewrite H in H6. constructor. 2 : constructor.
+      subst old_value.
+      assert (forall b, P4Arith.to_lbool (fst (P4Arith.BitArith.from_lbool b)) (snd (P4Arith.BitArith.from_lbool b)) = b)
+        as to_lbool_from_lbool by admit.
+      replace w with (fst (P4Arith.BitArith.from_lbool old_v))
+        by (unfold P4Arith.BitArith.from_lbool, fst; lia).
+      unfold P4Arith.to_loptbool.
+      rewrite to_lbool_from_lbool.
+      eapply exec_val_trans with (f := read_ndetbit). 3 : eassumption.
+      { red. sauto. }
+      constructor.
+      clear; induction old_v.
+      - constructor.
+      - constructor; auto. constructor.
+    }
+    2 : {
+      pose proof (P4Arith.BitArith.from_lbool_bound old_v).
+      unfold uncurry, P4Arith.BitArith.bound, P4Arith.BitArith.upper_bound in H4.
+      unfold P4Arith.BitArith.from_lbool in H4.
+      rewrite H0 in H4.
+      rewrite N2Z.id in H4.
+      subst old_value. simpl. lia.
+    }
+    clear H1.
+    destruct H2.
+    inv H1. inv H8. inv H9.
+    assert (sval_refine_sval_to_val_n_trans : forall v1 v2 v3,
+      sval_refine v1 v2 ->
+      sval_to_val read_ndetbit v2 v3 ->
+      sval_to_val read_ndetbit v1 v3). {
+      intros. eapply exec_val_trans; only 2, 3 : eassumption.
+      red; sauto.
+    }
+    inv H3. inv H10. inv H11.
+    eapply sval_refine_sval_to_val_n_trans in H6. 2 : eapply H8. clear H8.
+    eapply sval_refine_sval_to_val_n_trans in H5. 2 : eapply H7. clear H7.
+    split.
+    { eapply sval_to_val_bit_to_loptbool; eauto. }
+    { auto. }
+  }
+  clear H8.
+  destruct H1; subst.
+  split.
+  { inv H12. constructor. }
+  clear H12.
+  split.
+  { unfold ret_denote, ret_satisfies.
+    intros.
+    eapply exec_val_trans; only 2, 3 : eassumption.
+    clear; red; sauto.
+  }
+  split.
+  { constructor. }
+  { constructor.
+    2 : constructor.
+    simpl.
+    rewrite PathMap.get_set_same.
+    auto.
+  }
+Admitted.
+
 (* So the problem here is that, we need to define a rule for execute.
   And, should the ge constraint in spec for read and write be on the path quantifier? *)
 
@@ -168,7 +423,8 @@ The other is to find a way to prevent unfolding Extern typeclass in the computat
 Lemma Row_regact_insert_execute_body :
   fundef_satisfies_spec ge execute_fundef nil Row_regact_insert_execute_spec.
 Proof.
-  split.
+Admitted.
+(*   split.
   2 : {
     unfold func_modifies; intros.
     inv H.
@@ -346,7 +602,7 @@ Proof.
     rewrite PathMap.get_set_same.
     auto.
   }
-Admitted.
+Admitted. *)
 
 #[local] Hint Extern 5 (func_modifies _ _ _ _ _) => (apply Row_regact_insert_execute_body) : func_specs.
 (* #[local] Hint Extern 1 (list P4Type) => (exact (@nil _)) : func_specs. *)
@@ -376,14 +632,15 @@ Proof.
   unfold row_repr, row_reg_repr.
   normalize_EXT.
   step_call Row_regact_insert_execute_body.
-  2 : { entailer. }
-  { auto. }
+  3 : { entailer. }
+  { admit. }
+  { admit. }
   step.
   entailer.
   f_equal.
   unfold row_insert.
   list_solve.
-Qed.
+Admitted.
 
 Definition Row_fundef := Eval compute in
   force dummy_fundef (PathMap.get ["Bf2BloomFilterRow"; "apply"] (ge_func ge)).
